arm/proofs/aes_xts_decrypt_spec.ml
@@ -1,0 +1,21 @@
+use_file_raise_failure := true;;
+needs "common/aes.ml";;
+loadt "arm/proofs/aes_encrypt_spec.ml";;
+loadt "arm/proofs/aes_decrypt_spec.ml";;
+
+let pp_print_num fmt tm =
+  let n = dest_numeral tm in
+  pp_print_string fmt (string_of_num_hex n) in
+install_user_printer("pp_print_num",pp_print_num);;
+
+(*
+https://ieeexplore.ieee.org/stamp/stamp.jsp?tp=&arnumber=8637988
+
+*)
+
+let xts_init_tweak = new_definition
+  `xts_init_tweak (iv:int128) (key_schedule:int128 list) =
+    aes256_encrypt iv key_schedule`;;
+
+let aes256_xts_decrypt_round = new_definition
+  ``;;
